theories/SubstI3.v
@@ -161,14 +161,11 @@ Section subst.
           (forall u' t,
              nth_error tus' u' = Some t ->
              exists e, lookup (u + u') s = Some e) /\
-          exists sD',
-            substD tus tvs s' = Some sD' /\
-            exists eus' : list expr,
-              exists us' : hlist (fun t => hlist (typD nil) tus -> hlist (typD nil) tvs -> typD nil t) tus',
-                @hlist_build _ _ _ (fun t e => exprD' tus tvs e t) tus' eus' = Some us' /\
-                forall us vs,
-                  let us' := hlist_map (fun t (x : hlist (typD nil) tus -> hlist (typD nil) tvs -> typD nil t) => x us vs) us' in
-                  sD' us vs ->
+            exists sD',
+              substD tus tvs s' = Some sD' /\
+              forall us vs,
+                sD' us vs ->
+                exists us',
                   sD (hlist_app us us') vs
   }.
 
@@ -176,30 +173,6 @@ Section subst.
   Variable SubstOk_subst : SubstOk Subst_subst.
   Variable SubstUpdate_subst : SubstUpdate.
   Variable SubstUpdateOk_subst : SubstUpdateOk SubstUpdate_subst SubstOk_subst.
-
-  Theorem pull_sound_sem
-  : forall s s' u n,
-        pull u n s = Some s' ->
-        WellFormed_subst s ->
-        WellFormed_subst s' /\
-        forall tus tus' tvs sD,
-          u = length tus ->
-          n = length tus' ->
-          substD (tus ++ tus') tvs s = Some sD ->
-          exists sD',
-            substD tus tvs s' = Some sD' /\
-            exists eus' : list expr,
-              exists us' : hlist (fun t => hlist (typD nil) tus -> hlist (typD nil) tvs -> typD nil t) tus',
-                @hlist_build _ _ _ (fun t e => exprD' tus tvs e t) tus' eus' = Some us' /\
-                forall us vs,
-                  let us' := hlist_map (fun t (x : hlist (typD nil) tus -> hlist (typD nil) tvs -> typD nil t) => x us vs) us' in
-                  sD' us vs ->
-                  sD (hlist_app us us') vs.
-  Proof.
-    intros. eapply pull_sound in H; eauto.
-    intuition. specialize (H2 _ _ _ _ H H3 H4).
-    tauto.
-  Qed.
 
   Definition Subst_Extends (a b : T) : Prop :=
     forall tus tvs P Q,
@@ -220,6 +193,118 @@ Section subst.
         lookup u' s = Some e' ->
         mentionsU u' e = false
   }.
+
+  Fixpoint get_pull f l s : option (list expr) :=
+    match l with
+      | 0 => Some nil
+      | S l => match lookup f s with
+                 | None => None
+                 | Some e => match get_pull (S f) l s with
+                               | None => None
+                               | Some es => Some (e :: es)
+                             end
+               end
+    end.
+
+  Lemma list_ind_end
+  : forall T (P : list T -> Prop),
+      P nil ->
+      (forall x xs, P xs -> P (xs ++ x :: nil)) ->
+      forall xs, P xs.
+  Proof.
+    clear.
+    intros. rewrite <- rev_involutive.
+    induction (rev xs).
+    { simpl. assumption. }
+    { simpl. eauto. }
+  Qed.
+
+(*
+  Theorem pull_sound_sem
+  : forall s s' u n,
+        pull u n s = Some s' ->
+        WellFormed_subst s ->
+        WellFormed_subst s' /\
+        forall tus tus' tvs sD,
+          u = length tus ->
+          n = length tus' ->
+          substD (tus ++ tus') tvs s = Some sD ->
+          exists sD',
+            substD tus tvs s' = Some sD' /\
+            exists eus' : list expr,
+              exists us' : hlist (fun t => hlist (typD nil) tus -> hlist (typD nil) tvs -> typD nil t) tus',
+                @hlist_build _ _ _ (fun t e => exprD' tus tvs e t) tus' eus' = Some us' /\
+                forall us vs,
+                  let us' := hlist_map (fun t (x : hlist (typD nil) tus -> hlist (typD nil) tvs -> typD nil t) => x us vs) us' in
+                  sD' us vs ->
+                  sD (hlist_app us us') vs.
+  Proof.
+    intros. eapply pull_sound in H; eauto.
+    forward_reason. split; auto. intros.
+    specialize (H1 _ _ _ _ H2 H3 H4).
+    subst.
+    destruct H1. destruct H2 as [ ? [ ? ? ] ].
+    eexists; split; eauto.
+    consider (get_pull (length tus) (length tus') s).
+    { intros.
+      exists l.
+      Lemma get_pull_hlist_build
+      : forall s tus tus' tvs l,
+          get_pull (length tus) (length tus') s = Some l ->
+          exists us',
+            hlist_build (fun t : typ =>
+                           hlist (typD nil) (tus ++ tus') -> hlist (typD nil) tvs -> typD nil t)
+                        (fun (t : typ) (e : expr) => exprD' (tus ++ tus') tvs e t) tus' l =
+            Some us'.
+      Proof.
+        induction tus'; simpl.
+        { intros; inv_all; subst. inversion H0. }
+        { intros. forward.
+          inv_all. subst.
+          destruct n.
+          { rewrite Plus.plus_comm. simpl; congruence. }
+          { eapply IHt in H1. 2: instantiate (1 := n); omega.
+            replace (f + S n) with (S f + n) by omega. assumption. } }
+      Qed.
+      
+
+
+          eauto.
+        intro.
+        intros tus tus'.
+        eapply list_ind_end with (xs := tus').
+        { simpl. admit. }
+        { intros.
+          rewrite app_length in H1. simpl in H1. rewrite Plus.plus_comm in H1.
+          simpl in H1. forward.
+          inv_all; subst.
+          specialize (H0 
+        
+          
+
+induction tus'.
+        { simpl. admit. }
+        { 
+
+
+
+ }
+    { intro Hx. exfalso. clear - SubstOk_subst H H0 Hx.
+      generalize dependent (length tus).
+      induction tus'; simpl in *.
+      { congruence. }
+      { intros. specialize (IHtus' (S n)).
+        destruct (get_pull (S n) (length tus') s).
+        { forward.
+          specialize (H 0 a eq_refl).
+          destruct H. rewrite Plus.plus_0_r in H.
+          congruence. }
+        { eapply IHtus'; auto.
+          intros. specialize (H (S u') t H1).
+          replace (S n + u') with (n + S u') by omega.
+          assumption. } } }
+  Qed.
+*)
 
   Lemma substD_weakenU
   : forall tus tvs tus' s sD,
@@ -278,3 +363,41 @@ Section subst.
   Qed.
 
 End subst.
+
+
+(*
+
+    revert H2. revert H4. revert sD.
+    eapply rev_ind with (l := tus').
+    { simpl; intros.
+      clear H.
+      destruct H2 as [ ? [ ? ? ] ].
+      eexists; split; eauto.
+      exists nil. eexists; split; eauto.
+      intros. eapply H2 in H3.
+      destruct H3.
+      simpl. admit. }
+    { simpl; intros.
+      forward_reason.
+      eexists; split; eauto.
+      assert (nth_error (l ++ x :: nil) (length l) = Some x).
+      { rewrite ListNth.nth_error_app_R; eauto.
+        rewrite Minus.minus_diag. reflexivity. }
+      eapply H3 in H6.
+      destruct H6.
+      assert (exists sD', substD (tus ++ l) tvs s = Some sD'
+              /\ exists x,
+                   forall us us' vs,
+                     sD (hlist_app us (hlist_app us' (Hcons (x (hlist_app us us') vs) Hnil))) vs <->
+                     sD' (hlist_app us us') vs).
+      { admit. }
+      { forward_reason.
+        eapply H in H7; eauto.
+        { forward_reason.
+          exists (x5 ++ x1 :: nil).
+          eapply substD_lookup in H6; eauto.
+          forward_reason.
+          exists (hlist_app x6 (Hcons x8 Hnil)).
+
+  Qed.
+*)
